\documentclass{article}
\usepackage{amsmath}
\usepackage{amssymb}
\usepackage{amsthm}
\newtheorem{example}{Example}

\begin{document}

\begin{example}
$0=0$.
\end{example}

\begin{example}
$1+1=2$.
\end{example}

\begin{example}
$1\cdot 1=1$.
\end{example}

\begin{example}
$0<1$.
\end{example}

\begin{example}
$0\ne 1$.
\end{example}

\begin{example}
Let $x\in\mathbb{R}$. Then $x=x$.
\end{example}

\begin{example}
Let $x\in\mathbb{R}$. Then $x-x=0$.
\end{example}

\begin{example}
Let $x\in\mathbb{R}$. Then $x+x=2x$.
\end{example}

\begin{example}
Let $x\in\mathbb{R}$. Then $x^2\geq 0$.
\end{example}

\begin{example}
Let $x\in\mathbb{R}$. Assume $x\geq 1$. Then $x-1\geq 0$.
\end{example}

\begin{example}
Let $x\in\mathbb{R}$. Then $2(1+x)=2+2x$.
\end{example}

\begin{example}
Let $x\in\mathbb{R}$. Then $(1+x)x=x+x^2$.
\end{example}

\begin{example}
Let $x\in\mathbb{R}$. Then $(1+x)(1+x)=1+2x+x^2$.
\end{example}

\begin{example}
Let $x\in\mathbb{R}$. Let $y\in\mathbb{R}$. Then $(1+x)(1+y)=1+x+y+xy$.
\end{example}

\begin{example}
Let $x\in\mathbb{R}$. Let $y\in\mathbb{R}$. Then ${(x+y)}^2=x^2+2xy+y^2$.
\end{example}

\begin{example}
Let $x\in\mathbb{R}$. Let $y\in\mathbb{R}$. Then ${(x+y)}^3=x^3+3x^2y+3xy^2+y^3$.
\end{example}

\begin{example}
Let $x\in\mathbb{R}$. Let $y\in\mathbb{R}$. Then ${(x+y)}^4=x^4+4x^3y+6x^2y^2+4xy^3+y^4$.
\end{example}

\end{document}
